Removed more sorries

FraudProof/Games/FromBtoMTree.lean
@@ -17,7 +17,7 @@ structure ComputationTree (α ℍ : Type) where
 ----------------------------------------
 
 def dac_leaf_winning_condition {α ℍ : Type} [BEq ℍ]
-  [o : Hash α ℍ](hc : ℍ) (a : α)(_h : ℍ) : Bool := o.mhash a == hc
+  [o : Hash α ℍ](hc : ℍ) (a : α)(h : ℍ) : Bool := o.mhash a == hc ∧ h == hc
 
 def dac_node_winning_condition {ℍ : Type} [BEq ℍ]
   [m : HashMagma ℍ] (top hl hr : ℍ) : Bool := m.comb hl hr == top
@@ -47,7 +47,9 @@ def data_challenge_game{α ℍ : Type}
 
 theorem dac_winning_gen_chooser {α ℍ : Type}
     [hash : Hash α ℍ][HashMagma ℍ]
+    -- Hash equality depends on collision free hashes.
     [BEq ℍ][LawfulBEq ℍ]
+    --
     -- Public Information
     (pub_data : ABTree ℍ Unit)
     -- Players
@@ -62,8 +64,100 @@ theorem dac_winning_gen_chooser {α ℍ : Type}
     : data_challenge_game ⟨ pub_data , rev_res ⟩
          revealer (chooser.map (fun _ => ()) gen_chooser_opt)
          = Player.Chooser
-    := sorry
+    := by
+    revert hneq good_chooser ch_res chooser rev_res revealer
+    induction pub_data with
+    | leaf v =>
+      intros revealer rev_res chooser ch_res good_chooser hneq
+      simp
+      cases revealer with
+      | node _ _ _ => simp [treeCompArbGame]
+      | leaf rv =>
+        cases rv with
+        | none => simp [treeCompArbGame]
+        | some rv =>
+          simp [treeCompArbGame]
+          simp [winning_condition_player] at good_chooser
+          cases chooser with
+          | node _ _ _ => simp [winning_condition_player] at good_chooser
+          | leaf mcv =>
+            cases mcv with
+            | none => simp [winning_condition_player] at good_chooser
+            | some cv =>
+              simp [winning_condition_player] at good_chooser
+              unfold dac_leaf_winning_condition at *
+              -- Here, we do not need collision resistant, because we use logic.
+              -- I won't challenge a hash that it seems correct. Maybe the other
+              -- player only knows a collisition but not the real value.
+              simp at good_chooser
+              conv => lhs; simp; rw [Bool.and_comm]
+              simp
+              intro hrev_v
+              subst_eqs
+              tauto
+    | node v bl br HL HR =>
+      intros revealer rev_res chooser ch_res good_chooser hneq
+      simp
+      cases revealer with
+      | leaf _ => simp [treeCompArbGame]
+      | node mrev rev_left rev_right =>
+        cases mrev with
+        | none => simp [treeCompArbGame]
+        | some rev =>
+         simp [treeCompArbGame]
+         cases chooser with
+         | leaf _ =>
+           clear HL HR
+           simp [winning_condition_player] at good_chooser
+         | node mch ch_left ch_right =>
+           simp
+           cases mch with
+           | none =>
+             clear HL HR
+             simp [winning_condition_player] at good_chooser
+           | some ch =>
+             simp [winning_condition_player] at good_chooser
+             have gdac := good_chooser.1; simp [dac_node_winning_condition] at gdac
+             simp [gen_chooser_opt]
+             split
+             case h_1 x heq =>
+               apply Option.some.inj at heq
+               rw [ite_eq_iff] at heq
+               simp at heq
+               cases heq
+               case inl h =>
+                 simp [dac_node_winning_condition]
+                 subst_eqs
+                 rw [h.1,h.2] at hneq
+                 tauto
+               case inr h =>
+                 replace h := h.2
+                 rw [ite_eq_iff] at h
+                 simp at h
 
+             case h_2 x heq =>
+               apply Option.some.inj at heq
+               rw [ite_eq_iff] at heq
+               simp at heq
+               simp [data_challenge_game] at HL
+               apply HL
+               -- Proof obligations.
+               exact good_chooser.2.1
+               tauto
+
+             case h_3 x heq =>
+               apply Option.some.inj at heq
+               rw [ite_eq_iff] at heq
+               simp at heq
+               simp [data_challenge_game] at HR
+               apply HR
+               -- Proof obligations.
+               exact good_chooser.2.2
+               tauto
+
+             case h_4 x heq =>
+               clear HL HR
+               simp at heq
 
 @[simp]
 def treeArbitrationGame {α ℍ : Type}
